proof/refine/ARM/Reply_R.thy
@@ -16,6 +16,12 @@ defs replyUnlink_assertion_def:
 crunches setReplyTCB
   for pred_tcb_at'[wp]: "\<lambda>s. P (pred_tcb_at' proj test t s)"
   and tcb_at'[wp]: "\<lambda>s. P (tcb_at' t s)"
+  and ksReadyQueues[wp]: "\<lambda>s. P (ksReadyQueues s)"
+  and ksSchedulerAction[wp]: "\<lambda>s. P (ksSchedulerAction s)"
+  and valid_queues[wp]: "valid_queues"
+
+crunches getReplyTCB
+  for inv: "P"
 
 lemma replyUnlink_st_tcb_at':
   "\<lbrace>\<lambda>s. tcb_at' t s \<longrightarrow> (t' = t \<longrightarrow> P (P' Inactive)) \<and> (t' \<noteq> t \<longrightarrow> P (st_tcb_at' P' t' s))\<rbrace>
@@ -69,16 +75,10 @@ lemma replyUnlink_tcb_obj_at'_no_change:
    replyUnlink rptr tptr'
    \<lbrace>\<lambda>_ s. P (obj_at' Q tptr s)\<rbrace>"
   unfolding replyUnlink_def scheduleTCB_def rescheduleRequired_def
-            setReplyTCB_def getReplyTCB_def
+            setReplyTCB_def getReplyTCB_def updateReply_def
   apply (rule hoare_gen_asm)
-  apply (wpsimp wp: hoare_vcg_if_lift2 tcbSchedEnqueue_tcb_obj_at'_no_change set_reply'.get_inv
-                    isSchedulable_inv hoare_vcg_imp_lift setThreadState_tcb_obj_at'_no_change
-                    set_reply'.get_wp_rv_only threadSet_obj_at'_simple_strongest gts_wp'
-                    hoare_pre_cont[where a="isSchedulable x" and P="\<lambda>rv _. rv" for x]
-                    hoare_pre_cont[where a="getReply rptr" and P="\<lambda>rv s. \<not>tcb_at' (P rv) s" for P]
-              simp: o_def)
+  apply (wpsimp wp: setThreadState_tcb_obj_at'_no_change gts_wp')
   done
-
 
 lemma replyRemoveTCB_st_tcb_at'_sym_ref:
   "\<lbrace>(\<lambda>s. tcb_at' tptr s \<longrightarrow>
@@ -87,7 +87,7 @@ lemma replyRemoveTCB_st_tcb_at'_sym_ref:
       and (K (test Inactive))\<rbrace>
    replyRemoveTCB tptr
    \<lbrace>\<lambda>_. st_tcb_at' test tptr\<rbrace>"
-  unfolding replyRemoveTCB_def cleanReply_def
+  unfolding replyRemoveTCB_def cleanReply_def updateReply_def
   apply (rule hoare_gen_asm)
   supply set_reply'.get_wp[wp del] set_reply'.get_wp_state_only[wp] set_reply'.get_wp_rv_only[wp]
   apply (wpsimp wp: hoare_vcg_if_lift hoare_vcg_all_lift replyUnlink_st_tcb_at'_sym_ref
@@ -109,14 +109,458 @@ lemma replyRemoveTCB_st_tcb_at'_sym_ref:
   apply (clarsimp simp: obj_at'_def pred_tcb_at'_def)
   done
 
-lemma replyUnlink_valid_objs':
+lemma setReplyTCB_list_refs_of_replies':
+  "setReplyTCB tcb rptr \<lbrace>\<lambda>s. P (list_refs_of_replies' s)\<rbrace>"
+  unfolding setReplyTCB_def updateReply_def
+  apply wpsimp
+  apply (erule rsubst[where P=P])
+  apply (rule ext)
+  apply (clarsimp simp: list_refs_of_reply'_def obj_at'_def projectKO_eq
+                        list_refs_of_replies'_def opt_map_def
+                 split: option.splits)
+  done
+
+lemma setReply_valid_pde_mappings'[wp]:
+  "setReply p r \<lbrace>valid_pde_mappings'\<rbrace>"
+  unfolding valid_pde_mappings'_def setReply_def
+  apply (wpsimp wp: hoare_vcg_all_lift)
+  done
+
+lemma replyUnlink_valid_pspace'[wp]:
+  "replyUnlink rptr tptr \<lbrace>valid_pspace'\<rbrace>"
+  unfolding replyUnlink_def setReplyTCB_def getReplyTCB_def replyUnlink_assertion_def
+            updateReply_def
+  apply (wpsimp wp: sts'_valid_pspace'_inv hoare_vcg_imp_lift'
+              simp: valid_tcb_state'_def valid_pspace'_def)
+  apply normalise_obj_at'
+  apply (frule(1) reply_ko_at_valid_objs_valid_reply')
+  apply (clarsimp simp: valid_reply'_def)
+  done
+
+lemma replyUnlink_idle'[wp]:
+  "\<lbrace>valid_idle' and valid_pspace' and (\<lambda>s. tptr \<noteq> ksIdleThread s)\<rbrace>
+   replyUnlink rptr tptr
+   \<lbrace>\<lambda>_. valid_idle'\<rbrace>"
+  unfolding replyUnlink_def setReplyTCB_def replyUnlink_assertion_def updateReply_def
+  apply (wpsimp wp: getReplyTCB_wp hoare_vcg_imp_lift'
+              simp: pred_tcb_at'_def)
+  apply normalise_obj_at'
+  apply (frule(1) reply_ko_at_valid_objs_valid_reply'[OF _ valid_pspace_valid_objs'])
+  apply (clarsimp simp: valid_reply'_def)
+  done
+
+lemma replyUnlink_valid_queues[wp]:
+  "replyUnlink rptr tptr \<lbrace>valid_queues\<rbrace>"
+  unfolding replyUnlink_def replyUnlink_assertion_def getReplyTCB_def
+  apply (wpsimp wp: setThreadState_valid_queues' gts_wp' hoare_vcg_imp_lift')
+  done
+
+lemma setReplyTCB_replyNexts_replyPrevs[wp]:
+  "setReplyTCB tcb rptr \<lbrace>\<lambda>s. P (replyNexts_of s) (replyPrevs_of s)\<rbrace>"
+  unfolding setReplyTCB_def updateReply_def
+  apply wpsimp
+  apply (erule rsubst2[where P=P])
+   apply (clarsimp simp: ext opt_map_def list_refs_of_reply'_def obj_at'_def projectKO_eq
+                         map_set_def projectKO_opt_reply ARM_H.fromPPtr_def
+                  split: option.splits)+
+  done
+
+lemma cleanReply_replyNexts_replyPrevs[wp]:
+  "\<lbrace>\<lambda>s. P ((replyNexts_of s)(rptr := Nothing)) ((replyPrevs_of s)(rptr := Nothing))\<rbrace>
+   cleanReply rptr
+   \<lbrace>\<lambda>_ s. P (replyNexts_of s) (replyPrevs_of s)\<rbrace>"
+  unfolding cleanReply_def updateReply_def
+  apply (wpsimp wp: set_reply'.set_wp)
+  apply (erule rsubst2[where P=P])
+   apply (clarsimp simp: ext opt_map_def list_refs_of_reply'_def obj_at'_def projectKO_eq
+                         map_set_def projectKO_opt_reply ARM_H.fromPPtr_def
+                  split: option.splits)+
+  done
+
+lemma updateReply_valid_objs'_preserved_strong:
+  "\<lbrace>valid_objs' and (\<lambda>s. \<forall>r. valid_reply' r s \<longrightarrow> valid_reply' (upd r) s)\<rbrace>
+   updateReply rptr upd
+   \<lbrace>\<lambda>_. valid_objs'\<rbrace>"
+  unfolding updateReply_def
+  apply wpsimp
+  apply (frule(1) reply_ko_at_valid_objs_valid_reply')
+  apply clarsimp
+  done
+
+lemma updateReply_valid_objs'_preserved:
+  "\<lbrace>valid_objs' and K (\<forall>r s. valid_reply' r s \<longrightarrow> valid_reply' (upd r) s)\<rbrace>
+   updateReply rptr upd
+   \<lbrace>\<lambda>_. valid_objs'\<rbrace>"
+  apply (wpsimp wp: updateReply_valid_objs'_preserved_strong)
+  done
+
+lemma cleanReply_valid_objs'[wp]:
+  "cleanReply rptr \<lbrace>valid_objs'\<rbrace>"
+  unfolding cleanReply_def
+  apply (wpsimp wp: updateReply_valid_objs'_preserved
+              simp: valid_reply'_def)
+  done
+
+crunches cleanReply, updateReply
+  for valid_idle'[wp]: valid_idle'
+  and ct_not_inQ[wp]: ct_not_inQ
+  and sch_act_wf[wp]: "\<lambda>s. sch_act_wf (ksSchedulerAction s) s"
+  and valid_inQ_queues[wp]: valid_inQ_queues
+  and sch_act_not[wp]: "sch_act_not t"
+  and aligned'[wp]: pspace_aligned'
+  and distinct'[wp]: pspace_distinct'
+  and no_0_obj'[wp]: "no_0_obj'"
+  and cap_to': "ex_nonz_cap_to' t"
+
+crunches replyUnlink
+  for list_refs_of_replies'[wp]: "\<lambda>s. P (list_refs_of_replies' s)"
+  and replyNexts_replyPrevs[wp]: "\<lambda>s. P (replyNexts_of s) (replyPrevs_of s)"
+  and ct_not_inQ[wp]: ct_not_inQ
+  and ex_nonz_cap_to'[wp]: "(\<lambda>s. ex_nonz_cap_to' t s)"
+  and valid_irq_handlers'[wp]: valid_irq_handlers'
+  and valid_irq_states'[wp]: valid_irq_states'
+  and irqs_masked'[wp]: irqs_masked'
+  and ct_idle_or_in_cur_domain'[wp]: ct_idle_or_in_cur_domain'
+  and pspace_domain_valid[wp]: pspace_domain_valid
+  and gsUntypedZeroRanges[wp]: "\<lambda>s. P (gsUntypedZeroRanges s)"
+  and ksArchState[wp]: "\<lambda>s. P (ksArchState s)"
+  and gsMaxObjectSize[wp]: "\<lambda>s. P (gsMaxObjectSize s)"
+  and sch_act_not[wp]: "sch_act_not t"
+  (wp: crunch_wps)
+
+crunches replyRemoveTCB
+  for ctes_of[wp]: "\<lambda>s. P (ctes_of s)"
+  and aligned'[wp]: pspace_aligned'
+  and distinct'[wp]: pspace_distinct'
+  and ct_not_inQ[wp]: ct_not_inQ
+  and ct_idle_or_in_cur_domain'[wp]: ct_idle_or_in_cur_domain'
+  and cur_tcb'[wp]: "cur_tcb'"
+  and no_0_obj'[wp]: "no_0_obj'"
+  and it'[wp]: "\<lambda>s. P (ksIdleThread s)"
+  and ct'[wp]: "\<lambda>s. P (ksCurThread s)"
+  and ksCurDomain[wp]: "\<lambda>s. P (ksCurDomain s)"
+  and ksDomSchedule[wp]: "\<lambda>s. P (ksDomSchedule s)"
+  and ksInterruptState[wp]: "\<lambda>s. P (ksInterruptState s)"
+  and ksMachineState[wp]: "\<lambda>s. P (ksMachineState s)"
+  and ksDomScheduleIdx[wp]: "\<lambda>s. P (ksDomScheduleIdx s)"
+  and sch_act_simple[wp]: "sch_act_simple"
+  and valid_pde_mappings'[wp]: "valid_pde_mappings'"
+  and untyped_ranges_zero'[wp]: "untyped_ranges_zero'"
+  and ifunsafe'[wp]: "if_unsafe_then_cap'"
+  and global_refs'[wp]: "valid_global_refs'"
+  and valid_arch'[wp]: "valid_arch_state'"
+  and typ_at'[wp]: "\<lambda>s. P (typ_at' T p s)"
+  and vms'[wp]: "valid_machine_state'"
+  and valid_queues'[wp]: valid_queues'
+  and valid_queues[wp]: valid_queues
+  and valid_release_queue[wp]: valid_release_queue
+  and valid_release_queue'[wp]: valid_release_queue'
+  and cap_to': "ex_nonz_cap_to' t"
+  and pspace_domain_valid[wp]: pspace_domain_valid
+  (wp: crunch_wps hoare_vcg_if_lift
+   simp: pred_tcb_at'_def if_distribR if_bool_eq_conj)
+
+(* FIXME RT: move to...? *)
+lemma valid_mdb'_lift:
+  "(\<And>P. f \<lbrace>\<lambda>s. P (ctes_of s)\<rbrace>) \<Longrightarrow> f \<lbrace>valid_mdb'\<rbrace>"
+  unfolding valid_mdb'_def
+  apply simp
+  done
+
+lemma replyUnlink_valid_objs'[wp]:
   "replyUnlink rptr tptr \<lbrace>valid_objs'\<rbrace>"
-  apply (clarsimp simp: replyUnlink_def setReplyTCB_def getReplyTCB_def liftM_def updateReply_def)
-  apply (wpsimp wp: set_reply_valid_objs' hoare_vcg_all_lift gts_wp'
+  unfolding replyUnlink_def getReplyTCB_def
+  apply (wpsimp wp: updateReply_valid_objs'_preserved[where upd="replyTCB_update (\<lambda>_. tptrOpt)"
+                                                      for tptrOpt, folded setReplyTCB_def] gts_wp'
               simp: valid_tcb_state'_def)
-  apply (frule (1) ko_at_valid_objs'[where 'a=reply, simplified])
-   apply (clarsimp simp: projectKO_opt_reply split: kernel_object.splits)
-  apply (clarsimp simp: valid_obj'_def valid_reply'_def obj_at'_def)
+  apply (clarsimp simp: valid_reply'_def)
+  done
+
+lemma replyRemoveTCB_valid_pspace'[wp]:
+  "replyRemoveTCB tptr \<lbrace>valid_pspace'\<rbrace>"
+  unfolding replyRemoveTCB_def valid_pspace'_def cleanReply_def
+  supply set_reply'.set_wp[wp del] if_split[split del]
+  apply (wpsimp wp: valid_mdb'_lift updateReply_valid_objs'_preserved hoare_vcg_if_lift
+                    hoare_vcg_imp_lift gts_wp')
+  apply (clarsimp simp: valid_reply'_def if_bool_eq_conj if_distribR)
+  apply (case_tac "replyPrev ko = None"; clarsimp)
+   apply (drule(1) sc_ko_at_valid_objs_valid_sc'
+          , clarsimp simp: valid_sched_context'_def valid_sched_context_size'_def sc_size_bounds_def
+                           valid_reply'_def objBits_simps)+
+  done
+
+lemma updateReply_iflive':
+  "\<lbrace>if_live_then_nonz_cap' and K (\<forall>r. live_reply' (upd r) \<longrightarrow> live_reply' r)\<rbrace>
+   updateReply rptr upd
+   \<lbrace>\<lambda>_. if_live_then_nonz_cap'\<rbrace>"
+  apply (rule hoare_gen_asm)
+  unfolding if_live_then_nonz_cap'_def
+  apply (wpsimp wp: updateReply_cap_to' hoare_vcg_all_lift hoare_vcg_imp_lift'
+                    updateReply_wp_all)
+  apply (rename_tac ptr ko)
+  apply (case_tac "ptr = rptr")
+   apply clarsimp
+   apply (subst (asm) same_size_ko_wp_at'_set_ko'_iff)
+    apply (clarsimp simp: ko_wp_at'_def obj_at'_def projectKO_eq project_inject objBits_simps)
+   apply clarsimp
+   apply (erule allE, erule mp)
+   apply (erule allE, frule mp, assumption)
+   apply (clarsimp simp: ko_wp_at'_def obj_at'_def projectKO_eq project_inject)
+  apply (subst (asm) ko_wp_at'_set_ko'_distinct, assumption)
+   apply (clarsimp simp: ko_wp_at'_def obj_at'_def projectKO_eq project_inject)
+  apply fast
+  done
+
+lemma updateReply_valid_pspace'_strong:
+  "\<lbrace>valid_pspace' and (\<lambda>s. \<forall>r. valid_reply' r s \<longrightarrow> valid_reply' (upd r) s)\<rbrace>
+   updateReply rptr upd
+   \<lbrace>\<lambda>_. valid_pspace'\<rbrace>"
+  unfolding updateReply_def
+  apply (wpsimp wp: set_reply'.valid_pspace')
+  apply (frule(1) reply_ko_at_valid_objs_valid_reply'[OF _ valid_pspace_valid_objs'])
+  apply (clarsimp simp: valid_obj'_def)
+  done
+
+lemma updateReply_valid_pspace':
+  "\<lbrace>valid_pspace' and K (\<forall>r s. valid_reply' r s \<longrightarrow> valid_reply' (upd r) s)\<rbrace>
+   updateReply rptr upd
+   \<lbrace>\<lambda>_. valid_pspace'\<rbrace>"
+  apply (rule hoare_gen_asm)
+  apply (wpsimp wp: updateReply_valid_pspace'_strong)
+  done
+
+lemma setReplyTCB_None_iflive'[wp]:
+  "setReplyTCB None rptr \<lbrace>if_live_then_nonz_cap'\<rbrace>"
+  unfolding setReplyTCB_def
+  apply (wpsimp wp: updateReply_iflive' simp: live_reply'_def)
+  done
+
+lemma replyUnlink_iflive'[wp]:
+  "replyUnlink rptr tptr \<lbrace>if_live_then_nonz_cap'\<rbrace>"
+  unfolding replyUnlink_def
+  apply (wpsimp wp: setReplyTCB_None_iflive' gts_wp' getReplyTCB_wp)
+  done
+
+lemma cleanReply_iflive'[wp]:
+  "cleanReply rptr \<lbrace>if_live_then_nonz_cap'\<rbrace>"
+  unfolding cleanReply_def
+  apply (wpsimp wp: updateReply_iflive' simp: live_reply'_def)
+  done
+
+lemma replyRemoveTCB_iflive'[wp]:
+  "replyRemoveTCB tptr \<lbrace>if_live_then_nonz_cap'\<rbrace>"
+  unfolding replyRemoveTCB_def
+  apply (wpsimp wp: hoare_vcg_all_lift updateReply_iflive' hoare_vcg_if_lift hoare_vcg_imp_lift'
+                    gts_wp'
+         split_del: if_split)
+  apply (clarsimp simp: live_reply'_def)
+  apply (intro impI conjI allI
+         ; clarsimp simp: live_reply'_def pred_tcb_at'_def)
+   apply normalise_obj_at'
+   apply (rename_tac s sc reply tcb_reply_ptr prev_ptr next_ptr tcb)
+   apply (prop_tac "live_sc' sc")
+    apply (clarsimp simp: live_sc'_def)
+   apply (prop_tac "ko_wp_at' live' (theHeadScPtr (Some next_ptr)) s")
+    apply (clarsimp simp: ko_wp_at'_def obj_at'_def projectKO_eq project_inject)
+   apply (clarsimp simp: if_live_then_nonz_cap'_def)
+  apply normalise_obj_at'
+  apply (rename_tac s sc reply tcb_reply_ptr next_ptr tcb)
+  apply (prop_tac "live_sc' sc")
+   apply (clarsimp simp: live_sc'_def)
+  apply (prop_tac "ko_wp_at' live' (theHeadScPtr (Some next_ptr)) s")
+   apply (clarsimp simp: ko_wp_at'_def obj_at'_def projectKO_eq project_inject)
+  apply (clarsimp simp: if_live_then_nonz_cap'_def)
+  done
+
+lemma cleanReply_valid_pspace'[wp]:
+  "cleanReply rptr \<lbrace>valid_pspace'\<rbrace>"
+  unfolding cleanReply_def
+  apply (wpsimp wp: updateReply_valid_pspace' simp: live_reply'_def)
+  apply (clarsimp simp: valid_reply'_def)
+  done
+
+lemma decompose_list_refs_of_replies':
+  "list_refs_of_replies' s
+   = (\<lambda>r. get_refs ReplyPrev (replyPrevs_of s r) \<union> get_refs ReplyNext (replyNexts_of s r))"
+  apply (fastforce simp: opt_map_def map_set_def list_refs_of_reply'_def
+                  split: option.splits)
+  done
+
+lemma updateReply_replyNext_Nothing[wp]:
+  "\<lbrace>\<lambda>s. P ((replyNexts_of s)(rptr := Nothing)) (replyPrevs_of s)\<rbrace>
+   updateReply rptr (replyNext_update (\<lambda>_. Nothing))
+   \<lbrace>\<lambda>_ s. P (replyNexts_of s) (replyPrevs_of s)\<rbrace>"
+  unfolding updateReply_def
+  apply wpsimp
+  apply (erule rsubst2[where P=P])
+   apply (clarsimp simp: ext get_refs_def opt_map_def list_refs_of_reply'_def obj_at'_def
+                         projectKO_eq
+                  split: option.split)+
+  done
+
+lemma updateReply_replyPrev_Nothing[wp]:
+  "\<lbrace>\<lambda>s. P (replyNexts_of s) ((replyPrevs_of s)(rptr := Nothing))\<rbrace>
+   updateReply rptr (replyPrev_update (\<lambda>_. Nothing))
+   \<lbrace>\<lambda>_ s. P (replyNexts_of s) (replyPrevs_of s)\<rbrace>"
+  unfolding updateReply_def
+  apply wpsimp
+  apply (erule rsubst2[where P=P])
+   apply (clarsimp simp: ext get_refs_def opt_map_def list_refs_of_reply'_def obj_at'_def
+                         projectKO_eq
+                  split: option.split)+
+  done
+
+lemma cleanReply_list_refs_of_replies':
+  "\<lbrace>\<lambda>s. P ((list_refs_of_replies' s)(rptr := {}))\<rbrace>
+   cleanReply rptr
+   \<lbrace>\<lambda>_ s. P (list_refs_of_replies' s)\<rbrace>"
+  unfolding cleanReply_def decompose_list_refs_of_replies'
+  apply wpsimp
+  apply (erule rsubst[where P=P])
+  apply (rule ext)
+  apply (clarsimp simp: list_refs_of_reply'_def fun_upd_def)
+  done
+
+lemma isHead_to_head:
+  "isHead x = (\<exists>scPtr. x = Some (Head scPtr))"
+  "(\<forall>scPtr. y \<noteq> Head scPtr) = (\<exists>rPtr. y = Next rPtr)"
+  apply (clarsimp simp: isHead_def split: option.split reply_next.split)
+  apply (case_tac y; clarsimp)
+  done
+
+(* FIXME RT: remove. proved by MikiT *)
+lemma sym_refs_replyNext_replyPrev_proj:
+  "sym_refs (list_refs_of_replies' s') \<Longrightarrow>
+    replyNexts_of s' rp = Some rp' \<longleftrightarrow> replyPrevs_of s' rp' = Some rp"
+  sorry
+
+(* FIXME RT: remove. proved by MikiT *)
+lemma sym_refs_replyNext_None:
+  "\<lbrakk>sym_refs (list_refs_of_replies' s');
+    replyNexts_of s' rp = None \<rbrakk> \<Longrightarrow> \<forall>rp'. replyPrevs_of s' rp' \<noteq> Some rp"
+  sorry
+
+(* FIXME RT: remove. proved by MikiT *)
+lemma sym_refs_replyPrev_None:
+  "\<lbrakk>sym_refs (list_refs_of_replies' s');
+    replyPrevs_of s' rp = None \<rbrakk> \<Longrightarrow> \<forall>rp'. replyNexts_of s' rp' \<noteq> Some rp"
+  sorry
+
+lemma ks_reply_at'_repliesD:
+  "\<lbrakk>replies_of' s rptr = Some reply; sym_refs (list_refs_of_replies' s)\<rbrakk>
+   \<Longrightarrow> replyNexts_of s rptr = replyNext_of reply
+       \<and> (case replyNext_of reply of
+            Some next \<Rightarrow> replyPrevs_of s next = Some rptr
+          | None \<Rightarrow> \<forall>rptr'. replyPrevs_of s rptr' \<noteq> Some rptr)
+       \<and> replyPrevs_of s rptr = replyPrev reply
+       \<and> (case replyPrev reply of
+            Some prev \<Rightarrow> replyNexts_of s prev = Some rptr
+          | None \<Rightarrow> \<forall>rptr'. replyNexts_of s rptr' \<noteq> Some rptr)"
+  apply (prop_tac "replyNexts_of s rptr = replyNext_of reply
+                   \<and> replyPrevs_of s rptr = replyPrev reply ")
+   apply (clarsimp simp: opt_map_def)
+  apply (case_tac "replyNext_of reply"
+         ; case_tac "replyPrev reply"
+         ; clarsimp simp: sym_refs_replyNext_None sym_refs_replyPrev_None
+                          sym_refs_replyNext_replyPrev_proj)
+  done
+
+\<comment>\<open> Used to "hide" @{term "sym_refs o list_refs_of_replies'"} from simplification. \<close>
+definition protected_sym_refs :: "kernel_state \<Rightarrow> bool" where
+  "protected_sym_refs s \<equiv> sym_refs (list_refs_of_replies' s)"
+
+lemma replyRemoveTCB_sym_refs_list_refs_of_replies':
+  "replyRemoveTCB tptr \<lbrace>\<lambda>s. sym_refs (list_refs_of_replies' s)\<rbrace>"
+  unfolding replyRemoveTCB_def decompose_list_refs_of_replies'
+  supply if_cong[cong]
+  apply (wpsimp wp: cleanReply_list_refs_of_replies' hoare_vcg_if_lift hoare_vcg_imp_lift' gts_wp'
+                    haskell_assert_wp
+              simp: pred_tcb_at'_def
+         split_del: if_split)
+  unfolding decompose_list_refs_of_replies'[symmetric] protected_sym_refs_def[symmetric]
+  \<comment>\<open> opt_mapE will sometimes destroy the @{term "(|>)"} inside @{term replyNexts_of}
+      and @{term replyPrevs_of}, but we're using those as our local normal form. \<close>
+  supply opt_mapE[rule del]
+  apply (intro conjI impI allI)
+       \<comment>\<open> Our 6 cases correspond to various cases of @{term replyNext} and @{term replyPrev}.
+           We use @{thm ks_reply_at'_repliesD} to turn those cases into facts about
+           @{term replyNexts_of} and @{term replyPrevs_of}. \<close>
+       apply (all \<open>clarsimp simp: isHead_to_head
+                   , normalise_obj_at'\<close>)
+       apply (all \<open>drule(1) ks_reply_at'_repliesD[OF ko_at'_replies_of',
+                                                  folded protected_sym_refs_def]
+                   , clarsimp simp: projectKO_reply isHead_to_head\<close>)
+       \<comment>\<open> Now, for each case we can blow open @{term sym_refs}, which will give us enough new
+           @{term "(replyNexts_of, replyPrevs_of)"} facts that we can throw it all at metis. \<close>
+       apply (clarsimp simp: sym_refs_def split_paired_Ball in_get_refs
+              , intro conjI impI allI
+              ; metis sym_refs_replyNext_replyPrev_proj[folded protected_sym_refs_def] option.sel
+                      option.inject)+
+  done
+
+(* FIXME RT: move to...? *)
+lemma objBits_sc_only_depends_on_scRefills:
+  fixes sc :: sched_context
+    and upd :: "sched_context \<Rightarrow> sched_context"
+  assumes [simp]: "scRefills (upd sc) = scRefills sc"
+  shows "objBits (upd sc) = objBits sc"
+  apply (clarsimp simp: objBits_def objBitsKO_def)
+  done
+
+lemma replyRemoveTCB_valid_idle':
+  "\<lbrace>valid_idle' and valid_pspace'\<rbrace>
+   replyRemoveTCB tptr
+   \<lbrace>\<lambda>_. valid_idle'\<rbrace>"
+  unfolding replyRemoveTCB_def
+  apply (wpsimp wp: cleanReply_valid_pspace' updateReply_valid_pspace' hoare_vcg_if_lift
+                    hoare_vcg_imp_lift' gts_wp' setObject_sc_idle' haskell_assert_wp
+         split_del: if_split)
+  apply (clarsimp simp: valid_reply'_def pred_tcb_at'_def)
+  apply (intro conjI impI allI
+         ; simp?
+         , normalise_obj_at'?
+         , (solves \<open>clarsimp simp: valid_idle'_def idle_tcb'_def obj_at'_def isReply_def\<close>)?)
+     apply (frule(1) sc_ko_at_valid_objs_valid_sc'[OF _ valid_pspace_valid_objs']
+            , clarsimp simp: valid_sched_context'_def valid_sched_context_size'_def
+                             objBits_sc_only_depends_on_scRefills)+
+  done
+
+lemma replyUnlink_sch_act[wp]:
+  "\<lbrace>\<lambda>s. sch_act_wf (ksSchedulerAction s) s \<and> sch_act_not t s\<rbrace>
+   replyUnlink r t
+   \<lbrace>\<lambda>_ s. sch_act_wf (ksSchedulerAction s) s\<rbrace>"
+  apply (clarsimp simp: replyUnlink_def setReplyTCB_def getReplyTCB_def liftM_def)
+  by (wpsimp wp: sts_sch_act' hoare_drop_imp)
+
+lemma replyUnlink_weak_sch_act_wf[wp]:
+  "\<lbrace>\<lambda>s. weak_sch_act_wf (ksSchedulerAction s) s \<and> sch_act_not t s\<rbrace>
+   replyUnlink r t
+   \<lbrace>\<lambda>_ s. weak_sch_act_wf (ksSchedulerAction s) s\<rbrace>"
+  unfolding replyUnlink_def setReplyTCB_def getReplyTCB_def updateReply_def
+  by (wpsimp wp: hoare_vcg_imp_lift hoare_vcg_all_lift gts_wp'
+           simp: weak_sch_act_wf_def)
+
+lemma replyRemoveTCB_sch_act_wf:
+  "replyRemoveTCB tptr \<lbrace>\<lambda>s. sch_act_wf (ksSchedulerAction s) s\<rbrace>"
+  unfolding replyRemoveTCB_def
+  apply (wpsimp wp: gts_wp' haskell_assert_wp hoare_vcg_if_lift hoare_vcg_imp_lift'
+              simp: pred_tcb_at'_def
+         split_del: if_split)
+  apply normalise_obj_at'
+  apply (rename_tac tcb)
+  apply (case_tac "tcbState tcb"
+         ; clarsimp simp: isReply_def pred_tcb_at'_def)
+  apply (intro conjI impI allI
+         ; clarsimp simp: pred_tcb_at'_def obj_at'_def projectKO_eq project_inject)
+  done
+
+lemma replyRemoveTCB_invs':
+  "replyRemoveTCB tptr \<lbrace>invs'\<rbrace>"
+  unfolding invs'_def valid_state'_def
+  apply (wpsimp wp: replyRemoveTCB_sym_refs_list_refs_of_replies' replyRemoveTCB_valid_idle'
+                    valid_irq_node_lift valid_irq_handlers_lift' valid_irq_states_lift'
+                    irqs_masked_lift replyRemoveTCB_sch_act_wf
+              simp: cteCaps_of_def)
   done
 
 end
