proof/refine/ARM/Finalise_R.thy
@@ -2951,7 +2951,7 @@ lemma replyUnlink_makes_unlive:
         \<and> weak_sch_act_wf (ksSchedulerAction s) s\<rbrace>
    replyUnlink rptr tptr
    \<lbrace>\<lambda>_. ko_wp_at' (Not \<circ> live') rptr\<rbrace>"
-  apply (simp add: replyUnlink_def setReplyTCB_def)
+  apply (simp add: replyUnlink_def setReplyTCB_def updateReply_def)
   apply (wpsimp wp: setThreadState_Inactive_unlive set_reply'.set_wp gts_wp' getReplyTCB_wp)
   by (auto simp: ko_wp_at'_def obj_at'_def projectKOs is_aligned_def ps_clear_def
                  objBitsKO_def live'_def live_reply'_def weak_sch_act_wf_def pred_tcb_at'_def)
@@ -2960,9 +2960,10 @@ lemma cleanReply_makes_unlive:
   "\<lbrace>obj_at' (\<lambda>reply. replyTCB reply = None) rptr\<rbrace>
    cleanReply rptr
    \<lbrace>\<lambda>_. ko_wp_at' (Not \<circ> live') rptr\<rbrace>"
-  apply (simp add: cleanReply_def)
+  apply (simp add: cleanReply_def updateReply_def)
   apply (wpsimp wp: set_reply'.set_wp)
-  apply (auto simp: ko_wp_at'_def obj_at'_def projectKOs objBitsKO_def live_reply'_def)
+  apply (auto simp: ko_wp_at'_def obj_at'_def projectKOs objBitsKO_def live_reply'_def
+                    ps_clear_upd'[simplified fun_upd_def])
   done
 
 lemma replyClear_makes_unlive:
@@ -3566,7 +3567,7 @@ crunches setThreadState
 
 lemma replyUnlink_valid_reply'[wp]:
   "replyUnlink replyPtr tcbPtr \<lbrace>valid_reply' reply\<rbrace>"
-  apply (clarsimp simp: replyUnlink_def getReplyTCB_def liftM_def setReplyTCB_def)
+  apply (clarsimp simp: replyUnlink_def getReplyTCB_def liftM_def setReplyTCB_def updateReply_def)
   apply (wpsimp wp: set_reply'.set_wp gts_wp')
   by (auto simp: valid_reply'_def obj_at'_def projectKOs objBitsKO_def valid_bound_obj'_def
           split: option.splits)
@@ -3814,7 +3815,6 @@ lemma finaliseCapTrue_standin_valid_inQ_queues[wp]:
    \<lbrace>\<lambda>_. valid_inQ_queues\<rbrace>"
   unfolding finaliseCapTrue_standin_def Let_def
   apply (wpsimp wp: getReplyTCB_wp)
-  apply (simp add: obj_at'_def inQ_def)
   done
 
 crunches isFinalCapability
